theories/Prelude.v
@@ -1,4 +1,4 @@
-From Coq Require Export Nat List String Morphisms Relations Program.Equality Lia.
+From Coq Require Export Bool Nat List String Morphisms Relations Program.Equality Lia.
 From Ltac2 Require Export Ltac2.
 From Equations Require Export Equations.
 Export ListNotations.
